# Problem 1

## 1.

```pseudocode
function GetBoundary(P)
	bound1 = 1
	bound2 = 2
	n = P.len
	for i from 3 to n:
		query_result = PancakeGodOracle(P, bound1, bound2, i)
		if query_result == i:
			continue
		else if query_result == bound1:
			bound1 = i
		else if query_result == bound2:
			bound2 = i
	return bound1, bound2
```

Query is done for `n-2` times, therefore the query complexity is $O(n)$

---

## 2.

```pseudocode
/*
A[:-1] means the whole array A except the last element
A[2:] means the whole array A element except the first element
*/
function SortPancakes(P)
	n = P.len
	left_bound, right_bound = GetBoundary(P)
	swap(P, 1, left_bound); swap(P, n, right_bound)
	function QSort(P)
		m = P.len
		if m <= 2:
			return P
		else:
			pivot = random(2, m-1)
			l_pt = array(P[1]); r_pt = array(P[pivot])
			for i from 2 to m-1 except pivot:
				query = PancakeGodOracle(P, 1, pivot, i)
				if query == i:
					l_pt.append(P[i])
				else: 
					r_pt.append(P[i])
			l_pt.append(P[pivot]); r_pt.append(P[m])
			/* pivot will be in both l_pt and r_pt, so remove it when returning value */
			return QSort(l_pt)[:-1] + P[pivot] + QSort(r_pt)[2:]
	P = QSort(P)
```

My implementation is a pancake variation of quicksort. The recursion depth on average would be $O(\log n)$, and in each depth the query complexity is $O(n)$, therefore the total query complexity is $O(n\log n)$

---

## 3.

```pseudocode
function InsertPancake(L, new_pancake)
	l = 1; r = L.len
	L.append(new_pancake)
	new_p = L.len
	final_pos = -1
	while l < r:
		mid = floor((l+r)/2)
		query = PancakeGodOracle(P, l, mid, new_p)
		if query == new_p:
			r = mid-1
		else:
			l = mid+1
	final_pos = l
	for i from final_pos to L.len-1
		swap(L, i, L.len)
```

My implementation is a pancake variation of binary search. The query complexity can be easily found to be $O(\log n)$

---

## 4.

```pseudocode
/* A[1:i+1] means the array A from first element to i-th element */
function SortPancakesAgain(P)
	for i from 2 to P.len
		InsertPancake(P[1:i+1], P[i])
```

`InsertPancake()` runs `n` times, therefore the query complexity is $O(n\log n)$

---

## 5.

**Skipped**

---

## 6.

For $n=1$,  `P`is already in descending order and `ELF-SORT()` does nothing to `P`.

For $n=2$, if `P[2] > P[1]`, they will be swapped and then `P` is in descending order.

For $n=3$, the code would look like:

```
ELF-SORT(P, 1, 2)
ELF-SORT(P, 2, 3)
ELF-SORT(P, 1, 2)
```
The first two line moves the smallest element in `P` to the end, and the last line sorts `P[1]`and `P[2]`. `P` will be in descending order.

Assume that $\forall \ n \le k$, `ELF-SORT(P, 1, n)` sorts `P[1]` to `P[n]` in descending order. As shown above, this is true $\forall \ n \le 3$.

`ELF-SORT(P, 1+t, n+t)` also sorts `P[1+t]` to `P[n+t]` in descending order because it's just a shift on `P`.

For $n=k+1$, the code would look like:

```
Delta = floor((k+1)/3)
ELF-SORT(P, 1, k+1 - Delta)
ELF-SORT(P, 1 + Delta, k+1)
ELF-SORT(P, 1, k+1 - Delta)
```

Because we are only considering $n \ge 4$ in this part, `Delta` or $\Delta$ is always larger then $1$. Therefore all those three `ELF-SORT()` would sort the respective range in descending order.

The first two `ELF-SORT()` will sort the least $\frac{n}{3}$ element to the correct place, and the last one will sort the first $\frac{2n}{3}$ elements to the correct place. Therefore `P` is sorted in descending order.

Since `ELF-SORT(P, 1, n)` works for $n=1,2,3$, and if for $n=k$ `ELF-SORT` works, it would also work for $n=k+1$. By mathematical induction, `ELF-SORT(P, 1, n)` sorts `P` in descending order $\forall \ n \in \N$.

---

## 7.

For $n \ge 3$, the code would look like:

```
Delta = floor(n/3)
ELF-SORT(P, 1, n - Delta)
ELF-SORT(P, 1 + Delta, n)
ELF-SORT(P, 1, n - Delta)
```

From this, it's obvious that $T(n) = 3T(\frac{2}{3}n) + \Theta(1)$, because `floor()` runs at constant time

For $n = 2$, the running time is the time of two comparisons and a swap, which is $\Theta(1)$.

For $n = 1$, the running time is the time of two comparisons, which is $\Theta(1)$.

---

## 8.

By the recurrence relation we have:
$$
\begin{split}
T(n) & = 3^1T((\frac{2}{3})^1n) + \Theta(1) \\
3^1T((\frac{2}{3})^1n) & = 3^2T((\frac{2}{3})^2n) + 3^1\Theta(1) \\
3^2T((\frac{2}{3})^2n) & = 3^3T((\frac{2}{3})^3n) + 3^2\Theta(1) \\
& \cdots \\
3^{k-1}T((\frac{2}{3})^{k-1}n) & = 3^kT(1) + 3^{k-1}\Theta(1) \ \or \ 3^kT(2) + 3^{k-1}\Theta(1) \\
\end{split}
$$
Summing all $k$ equations and replacing $T(1)$ and $T(2)$ with $\Theta(1)$ yields:
$$
\begin{split}
T(n) & = 3^k\Theta(1) + \sum_{i=0}^{k-1} 3^i \cdot \Theta(1) \\
& = \sum_{i=0}^{k} 3^i \cdot \Theta(1) \\
& = \frac{3^{k+1} - 1}{3-1} \\
& = \frac{3}{2} 3^k - \frac{1}{2}
\end{split}
$$
And because $k = \lfloor \log_{\frac{3}{2}}n  \rfloor$, we have:
$$
\begin{split}
T(n) & = \frac{3}{2} 3^k - \frac{1}{2} \\
& = \frac{3}{2} 3^{\lfloor \log_{1.5}n  \rfloor} - \frac{1}{2} \\
& \le \frac{3}{2} 3^{1+\log_{1.5}n} - \frac{1}{2} \\
\frac{3}{2} 3^{1+\log_{1.5}n} - \frac{1}{2} & = \frac{9}{2} n^{\log_{1.5}3} - \frac{1}{2} \\
& \le \frac{9}{2} n^3
\end{split}
$$
Choose $n_0 = 1$ and $c=\frac{9}{2}$, we have:
$$
\forall \ n \ge n_0 = 1, \\
\begin{split}
T(n) & \le \frac{3}{2} 3^{1+\log_{1.5}n} - \frac{1}{2} \\
& \le \frac{9}{2} n^3 \\
& = c \cdot n^3 \\
\Rightarrow T(n) & = O(n^3) 
\end{split}
$$

---

